almost proven infering_on_free_vars, remain on_free_vars admissions

pcuic/theories/bidirectional/BDStrengthening.v
@@ -3,9 +3,9 @@ From Coq Require String.
 From MetaCoq.Template Require Import config utils monad_utils.
 From MetaCoq.PCUIC Require Import PCUICAst PCUICAstUtils PCUICInduction
   PCUICLiftSubst PCUICUnivSubst PCUICEquality PCUICUtils
-  PCUICPosition PCUICTyping PCUICSigmaCalculus PCUICRename PCUICOnFreeVars PCUICClosed PCUICConfluence PCUICSpine PCUICInductiveInversion.
+  PCUICPosition PCUICTyping PCUICSigmaCalculus PCUICRename PCUICOnFreeVars PCUICClosed PCUICConfluence PCUICSpine PCUICInductiveInversion PCUICParallelReductionConfluence.
 
-From MetaCoq.PCUIC Require Import BDEnvironmentTyping BDTyping.
+From MetaCoq.PCUIC Require Import BDEnvironmentTyping BDTyping BDToPCUIC BDFromPCUIC.
 
 Require Import ssreflect ssrbool.
 Require Import Coq.Program.Equality.
@@ -24,6 +24,28 @@ Proof.
       /on_free_vars_decl /test_decl /=. ring.
     rewrite on_free_vars_ctx_app /= IHΔ !lengths /= shiftnP_add on_free_vars_ctx_tip /= 
      /on_free_vars_decl /test_decl /=. ring.
+Qed.
+
+Lemma on_free_vars_case_predicate_context `{checker_flags} Σ ci mdecl idecl p P :
+  wf Σ ->
+  declared_inductive Σ ci mdecl idecl ->
+  forallb (on_free_vars P) (pparams p) ->
+  wf_predicate mdecl idecl p ->
+  All2 (compare_decls eq eq) (pcontext p) (ind_predicate_context ci mdecl idecl) ->
+  on_free_vars_ctx P (case_predicate_context ci mdecl idecl p).
+Proof.
+  intros.
+  rewrite /case_predicate_context /case_predicate_context_gen /pre_case_predicate_context_gen /inst_case_context.
+  erewrite <- on_free_vars_map2_cstr_args.
+  2: rewrite fold_context_k_length !map_length ; eapply All2_length ; tea.
+  apply on_free_vars_ctx_subst_context.
+  2: by rewrite forallb_rev.
+  rewrite on_free_vars_subst_instance_context List.rev_length.
+  apply closedn_ctx_on_free_vars_shift.
+  replace #|pparams p| with (context_assumptions (ind_params mdecl)).
+  1: eapply closed_ind_predicate_context ; tea ; eapply declared_minductive_closed ; eauto.
+  erewrite wf_predicate_length_pars ; tea.
+  eapply PCUICDeclarationTyping.onNpars, PCUICWeakeningEnv.on_declared_minductive ; eauto.
 Qed.
 
 Section OnFreeVars.
@@ -55,9 +77,13 @@ Section OnFreeVars.
   Let PΓ (Γ : context) :=
     True.
 
-  Theorem bidirectional_on_free_vars : env_prop_bd Σ Pcheck Pinfer Psort Pprod Pind PΓ.
+  Let PΓ_rel (Γ Γ' : context) := True.
+
+  Theorem bidirectional_on_free_vars : env_prop_bd Σ Pcheck Pinfer Psort Pprod Pind PΓ PΓ_rel.
   Proof.
     apply bidir_ind_env.
+
+    - constructor.
 
     - constructor.
 
@@ -113,18 +139,8 @@ Section OnFreeVars.
         rewrite test_context_k_closed_on_free_vars_ctx -closedn_ctx_on_free_vars in Hctx.
         apply /andP ; split.
         2: by rewrite case_predicate_context_length.
-        rewrite /predctx /case_predicate_context /case_predicate_context_gen /pre_case_predicate_context_gen /inst_case_context.
-        erewrite <- on_free_vars_map2_cstr_args.
-        2: rewrite fold_context_k_length !map_length ; eapply All2_length ; tea.
-        apply on_free_vars_ctx_subst_context.
-        2: by rewrite forallb_rev.
-        rewrite on_free_vars_subst_instance_context List.rev_length.
-        apply closedn_ctx_on_free_vars_shift.
-        replace #|pparams p| with (context_assumptions (ind_params mdecl)).
-        1: eapply closed_ind_predicate_context ; tea ; eapply declared_minductive_closed ; eauto.
-        erewrite wf_predicate_length_pars ; tea.
-        eapply PCUICDeclarationTyping.onNpars, PCUICWeakeningEnv.on_declared_minductive ; eauto.
-
+        eapply on_free_vars_case_predicate_context ; eassumption.
+        
       + rewrite forallb_app.
         apply /andP ; split.
         2: by rewrite /= andb_true_r.
@@ -175,18 +191,604 @@ Section OnFreeVars.
 
   Qed.
 
+  Lemma infering_on_free_vars P Γ t T :
+    on_ctx_free_vars P Γ ->
+    on_free_vars P t ->
+    Σ ;;; Γ |- t ▹ T ->
+    on_free_vars P T.
+  Proof.
+    intros.
+    edestruct bidirectional_on_free_vars as (_&_&_&p&_).
+    eapply p ; eauto.
+  Qed.
 
+  Lemma infering_prod_on_free_vars P Γ t na A B :
+    on_ctx_free_vars P Γ ->
+    on_free_vars P t ->
+    Σ ;;; Γ |- t ▹Π (na,A,B) ->
+    on_free_vars P A × on_free_vars (shiftnP 1 P) B.
+  Proof.
+    intros.
+    eapply bidirectional_on_free_vars ; eauto.
+  Qed.
 
-Lemma All_sigT {A B : Type} (P : A -> B -> Type) l :
-  All (fun x => ∑ y, P x y) l ->
-  ∑ l', All2 P l l'.
+End OnFreeVars.
+
+Lemma on_free_vars_type `{checker_flags} P Σ (wfΣ : wf Σ.1) Γ t T :
+  on_ctx_free_vars P Γ ->
+  on_free_vars P t ->
+  Σ ;;; Γ |- t : T ->
+  ∑ T', on_free_vars P T' × Σ ;;; Γ |- t : T'.
 Proof.
-  induction 1.
-  1: eexists ; constructor.
-  destruct p, IHX.
-  eexists.
-  by constructor ; eauto.
+  intros oΓ ot ty.
+  assert (wf_local Σ Γ) by (eapply typing_wf_local ; tea). 
+  apply typing_infering in ty as [T' []] ; tea.
+  exists T' ; split.
+  - edestruct bidirectional_on_free_vars as (_&_&_&?&_).
+    all: eauto.
+  - by apply infering_typing.
 Qed.
+
+Definition unlift_renaming n k i := if i <? k then i else if i <? k + n then 0 else i - n.
+Definition unlift n k := rename (unlift_renaming n k).
+
+Lemma lift_unlift n k : (unlift_renaming n k) ∘ (lift_renaming n k) =1 ren_id .
+Proof.
+  intros i.
+  rewrite /unlift_renaming /lift_renaming /ren_id.
+  repeat match goal with
+    | |- context [?x <? ?y] => destruct (Nat.ltb_spec0 x y) ; cbn
+    | |- context [?x <=? ?y] => destruct (Nat.leb_spec0 x y) ; cbn
+    | _ : context [?x <=? ?y] |- _ => destruct (Nat.leb_spec0 x y) ; cbn in *
+  end.
+  all: try congruence ; try lia.
+Qed.
+
+Corollary lift_unlift_term {n k} t : unlift n k (lift n k t) = t.
+Proof.
+  by rewrite lift_rename /unlift rename_compose lift_unlift rename_ren_id.
+Qed.
+
+(* Lemma shift_cond (P : nat -> bool) f f' :
+  (forall i, P i -> f i = f' i) ->
+  forall i n,
+  shiftnP n P i -> shiftn n f i = shiftn n f' i.
+Proof.
+  rewrite /shiftn /shiftnP.
+  intros H i n ?.
+  destruct (i <? n) ; cbn in * ; auto.
+  by rewrite H.
+Qed.
+
+Lemma cond_rename_ext (P : nat -> bool) f f' t:
+  (forall i, P i -> f i = f' i) ->
+  on_free_vars P t ->
+  rename f t = rename f' t.
+Proof.
+  intros H HP.
+  induction t using term_forall_list_ind in f, f', P, H, HP |- * ;
+  intros; cbn in |- *; try easy.
+  all: try solve [f_equal ; try rewrite H ; easy].
+  all: cbn in HP ;
+    repeat match goal with
+    | H : is_true (_ && _) |- _ => move: H => /andP [? ?]
+    | H : is_true (forallb _ _) |- _ => move: H => /forallb_All ?
+    end.
+  all: f_equal ; eauto.
+  - apply All_map_eq.
+    eapply All_mix in X ; tea.
+    eapply All_impl ; tea.
+    intros ? [] ; easy.
+  - eapply IHt2 ; eauto.
+    intros.
+    eapply shift_cond ; eauto.
+  - eapply IHt2 ; eauto.
+    intros.
+    eapply shift_cond ; eauto.
+  - eapply IHt3 ; eauto.
+    intros.
+    eapply shift_cond ; eauto.
+  - rewrite /rename_predicate.
+    destruct X as (IHpar&?&IHret).
+    f_equal.
+    + apply All_map_eq.
+      eapply All_mix in IHpar ; tea.
+      eapply All_impl ; tea.
+      intros ? [] ; easy.
+    + eapply IHret ; tea.
+      intros.
+      eapply shift_cond ; eauto.
+  - apply All_map_eq.
+    eapply All_mix in X0 ; tea.
+    eapply All_impl ; tea.
+    intros ? [i [? e]].
+    move: i => /andP [? ?].
+    rewrite /map_branch_shift.
+    f_equal.
+    eapply e ; tea.
+    intros.
+    eapply shift_cond ; eauto.
+  - apply All_map_eq.
+    eapply All_mix in X ; tea.
+    eapply All_impl ; tea.
+    intros ? [i [e e']].
+    move: i => /andP [? ?].
+    rewrite /map_def.
+    f_equal.
+    + eapply e ; eauto.
+    + eapply e' ; eauto.
+      intros. eapply shift_cond ; eauto.
+  - apply All_map_eq.
+    eapply All_mix in X ; tea.
+    eapply All_impl ; tea.
+    intros ? [i [e e']].
+    move: i => /andP [? ?].
+    rewrite /map_def.
+    f_equal.
+    + eapply e ; eauto.
+    + eapply e' ; eauto.
+      intros. eapply shift_cond ; eauto.
+Qed. *)
+
+Lemma urenaming_strengthen P Γ Δ decl :
+  urenaming (strengthenP #|Δ| 1 P) (Γ,,,Δ) (Γ ,, decl ,,, lift_context 1 0 Δ) (unlift_renaming 1 #|Δ|).
+Proof.
+  rewrite <- PCUICWeakening.rename_context_lift_context.
+  intros i decl' pi nthi.
+  rewrite /strengthenP in pi.
+  destruct (Nat.ltb_spec0 i #|Δ|) as [iΔ|iΔ].
+  - rewrite nth_error_app_context_lt in nthi.
+    1: by rewrite fold_context_k_length.
+    rewrite nth_error_rename_context in nthi.
+    apply option_map_Some in nthi as [decl'' []].
+    subst.
+    eexists ; split ; [idtac|split ; [idtac|split]].
+    + rewrite /unlift_renaming.
+      move: (iΔ) => /Nat.ltb_spec0 ->.
+      rewrite nth_error_app_context_lt //.
+      eassumption.
+    + reflexivity.
+    + rewrite /= rename_compose.
+      apply rename_proper ; auto.
+      intros x.
+      rewrite /rshiftk /shiftn /unlift_renaming /lift_renaming.
+      repeat match goal with
+        | |- context [?x <? ?y] => destruct (Nat.ltb_spec0 x y) ; cbn in *
+        | |- context [?x <=? ?y] => destruct (Nat.leb_spec0 x y) ; cbn in *
+        | _ : context [?x <? ?y] |- _ => destruct (Nat.ltb_spec0 x y) ; cbn in *
+        | _ : context [?x <=? ?y] |- _ => destruct (Nat.leb_spec0 x y) ; cbn in *
+      end.
+      all: try congruence ; try lia.
+    + cbn ; destruct (decl_body decl'') ; rewrite //=.
+      f_equal.
+      rewrite rename_compose.
+      apply rename_proper ; auto.
+      intros x.
+      rewrite /unlift_renaming /shiftn /lift_renaming.
+      repeat match goal with
+        | |- context [?x <? ?y] => destruct (Nat.ltb_spec0 x y) ; cbn in *
+        | |- context [?x <=? ?y] => destruct (Nat.leb_spec0 x y) ; cbn in *
+        | _ : context [?x <? ?y] |- _ => destruct (Nat.ltb_spec0 x y) ; cbn in *
+        | _ : context [?x <=? ?y] |- _ => destruct (Nat.leb_spec0 x y) ; cbn in *
+      end.
+      all: try congruence ; try lia.
+  - change (Γ ,, decl) with (Γ ,,, [decl]) in nthi.
+    rewrite -app_context_assoc /= in nthi.
+    destruct (Nat.ltb_spec0 i (#|Δ| + 1)) as [iΔ'|iΔ'] ; cbn in * ; [congruence|..].
+    apply Nat.nlt_ge in iΔ'.
+    rewrite nth_error_app_context_ge app_length /= rename_context_length // in nthi.
+    eexists ; repeat split.
+    + rewrite /unlift_renaming.
+      destruct (Nat.ltb_spec0 i #|Δ|) ; [lia|..].
+      destruct (Nat.ltb_spec0 i (#|Δ| + 1)) ; [lia|..].
+      rewrite nth_error_app_context_ge ; [lia|..].
+      rewrite -nthi.
+      f_equal.
+      lia.
+    + apply rename_proper ; auto.
+      intros x.
+      rewrite /unlift_renaming. 
+      repeat match goal with
+        | |- context [?x <? ?y] => destruct (Nat.ltb_spec0 x y) ; cbn in *
+        | |- context [?x <=? ?y] => destruct (Nat.leb_spec0 x y) ; cbn in *
+        | _ : context [?x <? ?y] |- _ => destruct (Nat.ltb_spec0 x y) ; cbn in *
+        | _ : context [?x <=? ?y] |- _ => destruct (Nat.leb_spec0 x y) ; cbn in *
+      end.
+      all: try congruence ; try lia.
+    + destruct (decl_body decl') ; rewrite //=.
+      f_equal.
+      apply rename_proper ; auto.
+      intros x.
+      rewrite /unlift_renaming.
+      repeat match goal with
+        | |- context [?x <? ?y] => destruct (Nat.ltb_spec0 x y) ; cbn in *
+        | |- context [?x <=? ?y] => destruct (Nat.leb_spec0 x y) ; cbn in *
+        | _ : context [?x <? ?y] |- _ => destruct (Nat.ltb_spec0 x y) ; cbn in *
+        | _ : context [?x <=? ?y] |- _ => destruct (Nat.leb_spec0 x y) ; cbn in *
+      end.
+      all: try congruence ; try lia.
+Qed.
+
+Axiom fix_guard_rename : forall P Σ Γ Δ mfix f,
+  urenaming P Γ Δ f ->
+  let mfix' := map (map_def (rename f) (rename (shiftn (List.length mfix) f))) mfix in
+  fix_guard Σ Δ mfix ->
+  fix_guard Σ Γ mfix'.
+
+Axiom cofix_guard_rename : forall P Σ Γ Δ mfix f,
+  urenaming P Γ Δ f ->
+  let mfix' := map (map_def (rename f) (rename (shiftn (List.length mfix) f))) mfix in
+  cofix_guard Σ Δ mfix ->
+  cofix_guard Σ Γ mfix'.
+
+Section BDRenaming.
+
+Context `{cf : checker_flags}.
+Context (Σ : global_env_ext).
+Context (wfΣ : wf Σ).
+
+Let Pinfer Γ t T :=
+  forall P Δ f,
+  urenaming P Δ Γ f ->
+  on_ctx_free_vars P Γ ->
+  on_free_vars P t ->
+  Σ ;;; Δ |- rename f t ▹ rename f T.
+
+Let Psort Γ t u :=
+  forall P Δ f,
+  urenaming P Δ Γ f ->
+  on_ctx_free_vars P Γ ->
+  on_free_vars P t ->
+  Σ ;;; Δ |- rename f t ▹□ u.
+
+Let Pprod Γ t na A B :=
+  forall P Δ f,
+  urenaming P Δ Γ f ->
+  on_ctx_free_vars P Γ ->
+  on_free_vars P t ->
+  Σ ;;; Δ |- rename f t ▹Π (na,rename f A,rename (shiftn 1 f) B).
+
+Let Pind Γ ind t u args :=
+  forall P Δ f,
+  urenaming P Δ Γ f ->
+  on_ctx_free_vars P Γ ->
+  on_free_vars P t ->
+  Σ ;;; Δ |- rename f t ▹{ind} (u, map (rename f) args).
+  
+
+Let Pcheck Γ t T :=
+  forall P Δ f,
+  urenaming P Δ Γ f ->
+  on_ctx_free_vars P Γ ->
+  on_free_vars P t ->
+  on_free_vars P T ->
+  Σ ;;; Δ |- rename f t ◃ rename f T.
+
+Let PΓ :=
+  All_local_env (lift_sorting (fun _ => Pcheck) (fun _ => Psort) Σ).
+
+Let PΓ_rel Γ Γ' :=
+  forall P Δ f,
+  urenaming P Δ Γ f ->
+  on_ctx_free_vars P Γ ->
+  on_free_vars_ctx P Γ' ->
+  wf_local_bd_rel Σ Δ (rename_context f Γ').
+
+(* Lemma wf_local_app_renaming P Γ Γ' Δ f:
+  on_ctx_free_vars P Γ ->
+  wf_local_bd Σ (Γ ,,, Δ) ->
+  PΓ (Γ ,,, Δ) ->
+  urenaming P Γ' Γ f ->
+  wf_local_bd Σ (Γ' ,,, rename_context f Δ).
+Proof.
+  intros hclo wfΓ hP u.
+  induction Δ in Γ, Γ', wfΓ, f, u, hP |- *.
+  - cbn in *.
+    red in hP.
+  
+  
+  - rewrite rename_context_snoc.
+    destruct a as [? [] ?] ; cbn in *.
+    + constructor ; cbn.
+      * eapply IHΔ ; tea.
+      * 
+
+  
+    rewrite rename_context_snoc /=.
+    constructor ; eauto.
+    eexists.
+    red in p.
+    eapply p ; eauto.
+    + eapply urenaming_context. 
+  
+    simpl. destruct t0 as [s Hs].
+    rewrite rename_context_snoc /=. constructor; auto.
+    red. simpl. exists s.
+    eapply (Hs P (Δ' ,,, rename_context f Γ0) (shiftn #|Γ0| f)).
+    split => //.
+    eapply urenaming_ext.
+    { len. now rewrite -shiftnP_add. }
+    { reflexivity. } now eapply urenaming_context.
+  - destruct t0 as [s Hs]. red in t1.
+    rewrite rename_context_snoc /=. constructor; auto.
+    * red. exists s.
+      apply (Hs P (Δ' ,,, rename_context f Γ0) (shiftn #|Γ0| f)).
+      split => //.
+      eapply urenaming_ext.
+      { len; now rewrite -shiftnP_add. }
+      { reflexivity. } now eapply urenaming_context.
+    * red. apply (t1 P). split => //.
+      eapply urenaming_ext. 
+      { len; now rewrite -shiftnP_add. }
+      { reflexivity. } now eapply urenaming_context.
+Qed. *)
+
+Theorem bidirectional_renaming : env_prop_bd Σ Pcheck Pinfer Psort Pprod Pind PΓ PΓ_rel.
+Proof.
+  apply bidir_ind_env.
+
+  - intros Γ wfΓ hΓ. red.
+    induction hΓ.
+    + constructor.
+    + constructor ; tea.
+      eexists ; eauto.
+    + constructor ; tea.
+      eexists ; eauto.
+
+  - intros Γ Γ' wfΓ' allΓ'. red. move => P Δ f hf hΓ hΓ'.
+    induction allΓ'.
+    + constructor.
+    + rewrite rename_context_snoc.
+      rewrite on_free_vars_ctx_snoc in hΓ'.
+      move: hΓ' => /andP [] ? ?.
+      constructor ; eauto.
+      1: by eapply IHallΓ' ; eauto.
+      eexists.
+      eapply s.
+      * eapply urenaming_context ; tea.
+      * rewrite on_ctx_free_vars_concat.
+        apply /andP ; split ; tea.
+        by rewrite on_free_vars_ctx_on_ctx_free_vars.
+      * eassumption.
+    + rewrite rename_context_snoc.
+      rewrite on_free_vars_ctx_snoc in hΓ'.
+      move: hΓ' => /andP [] ? /andP /= [] ? ?.
+      constructor ; eauto.
+      * by eapply IHallΓ' ; eauto.
+      * eexists.
+        eapply s.
+        1: eapply urenaming_context ; tea.
+        2: eauto.
+        rewrite on_ctx_free_vars_concat.
+        apply /andP ; split ; tea.
+        by rewrite on_free_vars_ctx_on_ctx_free_vars.
+      * eapply c.
+        1: eapply urenaming_context ; tea.
+        all: auto.
+        rewrite on_ctx_free_vars_concat.
+        apply /andP ; split ; tea.
+        by rewrite on_free_vars_ctx_on_ctx_free_vars.
+  
+  - intros Γ n decl isdecl P Δ f hf hΓ ht.
+    eapply hf in isdecl as h => //.
+    destruct h as [decl' [isdecl' [? [h1 h2]]]].
+    rewrite lift0_rename rename_compose h1 -lift0_rename.
+    econstructor. all: auto.
+
+  - intros. red. intros. cbn in *.
+    by constructor.
+    
+  - intros. red. move => P Δ f hf hΓ /= /andP [] ? ?.
+    econstructor ; eauto.
+    eapply X2 ; tea.
+    1: by apply urenaming_vass.
+    rewrite on_ctx_free_vars_snoc /=.
+    apply /andP ; split ; tea.
+    
+  - intros. red. move => P Δ f hf hΓ /= /andP [] ? ?.
+    econstructor ; eauto.
+    eapply X2 ; tea.
+    1: by apply urenaming_vass.
+    rewrite on_ctx_free_vars_snoc /=.
+    apply /andP ; split ; tea.
+
+  - intros. red. move => P Δ f hf hΓ /= /andP [] ? /andP [] ? ?.
+    econstructor ; eauto.
+    eapply X4 ; tea.
+    1: by apply urenaming_vdef.
+    rewrite on_ctx_free_vars_snoc.
+    repeat (apply /andP ; split ; tea).
+
+  - intros. red. move => P Δ f hf hΓ /= /andP [] ? ?.
+    rewrite rename_subst0 ; cbn.
+    econstructor ; eauto.
+    eapply X2 ; tea.
+    eapply infering_prod_on_free_vars.
+    4: eassumption.
+    all: assumption.
+
+  - intros. red. move => P Δ f hf hΓ /= _.
+    rewrite rename_subst_instance.
+    erewrite rename_closed.
+    2: by eapply declared_constant_closed_type ; tea.
+    econstructor ; tea.
+
+  - intros. red. move => P Δ f hf hΓ /= _.
+    rewrite rename_subst_instance.
+    erewrite rename_closed.
+    2: by eapply declared_inductive_closed_type ; tea.
+    econstructor ; tea.
+  
+  - intros. red. move => P Δ f hf hΓ /= _.
+    erewrite rename_closed.
+    2: by eapply declared_constructor_closed_type ; tea.
+    econstructor ; tea.
+
+  - intros. red. move => P Δ f hf hΓ /= /andP [] on_pars /andP [] ? /andP [] ? /andP [] ? /forallb_All on_brs.
+    rewrite rename_mkApps rename_it_mkLambda_or_LetIn map_app map_skipn /=.
+    rewrite rename_case_predicate_context // case_predicate_context_length // rename_predicate_preturn.
+    econstructor ; eauto.
+    + by eapply rename_wf_predicate.
+    + rewrite -rename_case_predicate_context ; tea.
+      eapply X1 ; tea.
+      eapply on_free_vars_case_predicate_context ; tea.
+    + eapply X3 ; tea.
+      * rewrite -rename_case_predicate_context //.
+        erewrite <- case_predicate_context_length ; tea.
+        apply urenaming_context ; assumption.
+      * erewrite <- case_predicate_context_length ; tea.
+        rewrite /predctx.
+        erewrite on_ctx_free_vars_concat.
+        apply /andP ; split ; tea.
+        rewrite on_free_vars_ctx_on_ctx_free_vars.
+        eapply on_free_vars_case_predicate_context ; tea.
+    + revert X7.
+      rewrite -{2}[subst_instance _ _](rename_closedn_ctx f 0).
+      { pose proof (declared_inductive_closed_params isdecl).
+        now rewrite closedn_subst_instance_context. }
+      rewrite rename_context_telescope rename_telescope_shiftn0 /=.
+      admit.
+    + rewrite /= /id -map_skipn -map_app.
+      eapply cumul_renameP in X8 ; tea.
+      * by rewrite !rename_mkApps /= in X8.
+      * rewrite on_free_vars_mkApps /=.
+        eapply All_forallb, bidirectional_on_free_vars ; tea.
+      * rewrite on_free_vars_mkApps /=.
+        rewrite forallb_app ; apply /andP ; split ; tea.
+        apply forallb_skipn.
+        eapply All_forallb, bidirectional_on_free_vars ; tea.
+    + by apply rename_wf_branches.
+    + eapply Forall2_All2 in H4.
+      eapply All2i_All2_mix_left in X9; eauto.
+      eapply All2i_All_mix_right in X9 ; eauto.
+      eapply All2i_nth_hyp in X9.
+      eapply All2i_map_right, (All2i_impl X9) => i cdecl br.
+      set (brctxty := case_branch_type _ _ _ _ _ _ _ _).
+      move=> [Hnth [ [wfbr [eqbctx [wfbctx [IHbctx [Hbod IHbod]]]]] /andP [on_ctx on_bod] ]].
+      rewrite -(rename_closed_constructor_body mdecl cdecl f).
+      { eapply (declared_constructor_closed (c:=(ci.(ci_ind),i))); eauto.
+        split; eauto. }
+      split; auto.
+      { simpl. rewrite -rename_cstr_branch_context //.
+        1:eapply (declared_inductive_closed_params isdecl).
+        rewrite rename_closedn_ctx //.
+        eapply closed_cstr_branch_context.
+        1:by eapply declared_minductive_closed ; eauto.
+        eapply (declared_constructor_closed (c:=(ci.(ci_ind),i))). split; tea.
+      }
+      cbn -[case_branch_type case_predicate_context].
+      rewrite case_branch_type_fst.
+      rewrite -rename_case_branch_context_gen //.
+      2-3:len.
+      1:exact (declared_inductive_closed_params isdecl).
+      1:rewrite (wf_branch_length wfbr) //.
+      1:rewrite (wf_predicate_length_pars H0).
+      1:erewrite declared_minductive_ind_npars ; eauto.
+      assert (on_free_vars_ctx P brctxty.1).
+      { rewrite test_context_k_closed_on_free_vars_ctx in on_ctx.        
+        admit. }
+      set (brctx' := rename_context f _).
+      split.
+      1:by eapply IHbctx ; eauto.
+      rewrite rename_case_branch_type //.
+      eapply IHbod.
+      * rewrite case_branch_type_fst /=.
+        relativize #|bcontext br| ; [eapply urenaming_context|] ; tea.
+        by rewrite case_branch_context_length.
+      * rewrite case_branch_context_length ; tea.
+        relativize (#|bcontext br|).
+        1: erewrite on_ctx_free_vars_concat.
+        2: rewrite case_branch_type_length //.
+        2: erewrite wf_branch_length ; eauto.
+        apply /andP ; split ; tea.
+        by rewrite on_free_vars_ctx_on_ctx_free_vars.
+      * rewrite case_branch_type_length //.
+        erewrite <- wf_branch_length ; eauto.
+      * rewrite case_branch_context_length //.
+        admit.
+  
+  - intros. red. move => P Δ f hf hΓ /= ?.
+    rewrite rename_subst0 /= rename_subst_instance map_rev List.rev_length.
+    erewrite rename_closedn.
+    2: rewrite H0 ; eapply declared_projection_closed_type ; tea.
+    econstructor ; eauto.
+    by rewrite map_length.    
+
+  - intros. red. move => P Δ f hf hΓ /= /forallb_All ht.
+    erewrite map_dtype.
+    econstructor.
+    + eapply fix_guard_rename ; tea.
+    + by rewrite nth_error_map H0 /=.
+    + eapply All_mix in X ; tea.
+      eapply All_map, All_impl ; tea.
+      move => ? [] /andP [] ? ? [] ? [] ? p.
+      rewrite -map_dtype.
+      eexists.
+      eapply p ; tea.
+    + eapply All_mix in X0 ; tea.
+      eapply All_map, All_impl ; tea.
+      move => ? [] /andP [] ? ? [] ? p.
+      rewrite -map_dbody -map_dtype rename_fix_context rename_context_length -(fix_context_length mfix) -rename_shiftn.
+      eapply p ; tea.
+      * rewrite -(fix_context_length mfix).
+        eapply urenaming_context ; tea.
+      * by apply on_ctx_free_vars_fix_context.
+      * rewrite -(Nat.add_0_r (#|mfix|)) fix_context_length.
+        apply on_free_vars_lift_impl.
+        by rewrite shiftnP0.
+    + by apply rename_wf_fixpoint. 
+
+  - intros. red. move => P Δ f hf hΓ /= /forallb_All ht.
+    erewrite map_dtype.
+    econstructor.
+    + eapply cofix_guard_rename ; tea.
+    + by rewrite nth_error_map H0 /=.
+    + eapply All_mix in X ; tea.
+      eapply All_map, All_impl ; tea.
+      move => ? [] /andP [] ? ? [] ? [] ? p.
+      rewrite -map_dtype.
+      eexists.
+      eapply p ; tea.
+    + eapply All_mix in X0 ; tea.
+      eapply All_map, All_impl ; tea.
+      move => ? [] /andP [] ? ? [] ? p.
+      rewrite -map_dbody -map_dtype rename_fix_context rename_context_length -(fix_context_length mfix) -rename_shiftn.
+      eapply p ; tea.
+      * rewrite -(fix_context_length mfix).
+        eapply urenaming_context ; tea.
+      * by apply on_ctx_free_vars_fix_context.
+      * rewrite -(Nat.add_0_r (#|mfix|)) fix_context_length.
+        apply on_free_vars_lift_impl.
+        by rewrite shiftnP0.
+    + by apply rename_wf_cofixpoint. 
+  
+  - intros. red. intros P Δ f hf ht.
+    econstructor ; eauto.
+    rewrite -/(rename f (tSort u)).
+    eapply red_rename ; tea.
+    eapply infering_on_free_vars ; tea.
+
+  - intros. red. intros P Δ f hf hΓ ht.
+    econstructor ; eauto.
+    rewrite -/(rename f (tProd na A B)).
+    eapply red_rename ; tea.
+    eapply infering_on_free_vars ; tea.
+
+  - intros. red. intros P Δ f hf hΓ ht.
+    econstructor ; eauto.
+    rewrite -/(rename f (tInd ind ui)) -rename_mkApps.
+    eapply red_rename ; tea.
+    eapply infering_on_free_vars ; tea.
+
+  - intros. red. intros P Δ f hf hΓ ht.
+    econstructor ; eauto.
+    eapply cumul_renameP ; tea.
+    eapply infering_on_free_vars.
+    4: eassumption.
+    all: assumption.
+
+Admitted.
+
 
 
 Lemma strengthenP_unlift (p : nat -> bool) n k t : 
